code/ecdsap256/Hacl.P256.fst
@@ -82,3 +82,7 @@ let ecp256dh_r result pubKey scalar = Hacl.Impl.P256.DH.ecp256dh_r result pubKey
 (* 
 let is_more_than_zero_less_than_order x =
   Hacl.Impl.P256.Signature.Common.isMoreThanZeroLessThanOrder x
+
+*)
+
+let getScalar #a scalar i = Hacl.Impl.P256.Core.getScalar #a scalar i 
