code/ecdsap256/Hacl.Impl.P256.LowLevel.fst
@@ -127,16 +127,6 @@ let load_buffer8 a0 a1 a2 a3 a4 a5 a6 a7  o =
   upd o (size 6) a6;
   upd o (size 7) a7
 
-(** This is unused *)
-inline_for_extraction noextract
-val copy_conditional_u64: a: uint64 -> b: uint64 -> mask: uint64 {uint_v mask = 0 \/ uint_v mask = pow2 64 - 1} -> 
-  Tot (r: uint64 {if uint_v mask = 0 then uint_v r = uint_v a else uint_v r = uint_v b})
-
-let copy_conditional_u64 a b mask = 
-  lemma_xor_copy_cond a b mask;
-  logxor a (logand mask (logxor a b))
-
-
 
 inline_for_extraction noextract
 val copy_conditional: out: felem -> x: felem -> mask: uint64{uint_v mask = 0 \/ uint_v mask = pow2 64 - 1} -> Stack unit 
